improved verification for transport

projectVampire/python/transportationManager.py
@@ -2,33 +2,100 @@ class transportationManager:
 
 	def __init__(self, location, sys):
 		self.locale = location # location of this transport manager
-		self.toSend = [] # blood that is to be sent
+		self._available = 0 # currently available accept spot
+		self._size = 10 # size of transportBuffer
+		self.toSend = [None for x in range(self._size)] # initialise to null
+		self.toDest = [-1 for x in range(self._size)] # initialise to non-valid dests
 		self.node = None
 		self._sys = sys
 
-	# Get blood
+	def _valid(self):
+		dstNull = (self.toDest != None)
+		sndNull = (self.toSend != None)
+		size    = (self._size > 0)
+		sizeDst = (self._size == len(self.toDest))
+		sizeSnd = (self._size == len(self.toSend))
+		avRange = (-1 <= self._available <= (self._size-1))
+		matchin = True
+		for i in range(self._size):
+			if (self.toSend[i] and (self.toDest[i] == -1)):
+				matchin = False
+		#print(dstNull,sndNull,size, sizeDst,sizeSnd,avRange,matchin)
+		return dstNull and sndNull and size and sizeDst and sizeSnd and avRange and matchin
 
 	def arrivalAccept(self, blood):
 		self.locale.accept(blood)
-		#self.locale.accept(blood)
 
 	def receive(self, blood, dest):
-		#print("Sending blood to ", dest.name)
-		if dest == None:
-			dest = self.getBloodDest(blood) 
-		# blood is to be sent
-		self.toSend.append([blood,dest])
-
-	# Add route to destinations
-	#def addRoute(self, location, route):
-	#    self.destinations[location] = route;
-
-	# Send blood to transportationRoute
-	def dispatchBlood(self):
-		#for tup in self.toSend:
+		old_DEST = self.toDest.copy()
+		old_SEND = self.toSend.copy()
+		assert self.toSend != None
+		assert self.toDest != None
 		for i in range(len(self.toSend)):
-			print('**Blood has been dispatched**')
-			self._sys.getRoutingSys().sendBlood(self.toSend.pop(i), self.node)
+			assert self.toSend[i] != blood
+		assert blood != None
+		assert self._valid()
+		if dest == None: # linking to dynamic routing
+			dest = self.getBloodDest(blood) 
+		assert dest != None
+
+		if self._available == self._size -1:
+			self._available = 0 
+		else:
+			self._available = self._available + 1
+		self.toSend[self._available] = blood
+		self.toDest[self._available] = dest
+
+		assert self._valid
+		assert 0 <= self._available < len(self.toSend)
+		assert 0 <= self._available < len(self.toDest)
+		for i in range(len(self.toSend)):
+			if i != self._available:
+				assert old_SEND[i] == self.toSend[i] 
+		for i in range(len(self.toDest)):
+			if i != self._available:
+				assert old_DEST[i] == self.toDest[i]
+
+	# Dispatch all blood stored in this manager
+	def dispatchBlood(self):
+		assert self._valid()
+		assert self.toSend != None
+		assert self.toDest != None
+		hasSendVals = False
+		for i in range(self._size):
+			if (self.toSend[i]):
+				hasSendVals = True
+		assert hasSendVals
+
+
+		i = 0
+		j = 0
+		while (i < len(self.toSend) and j < len(self.toDest)):
+
+			assert i == j
+			assert 0 <= i < len(self.toSend)
+			assert 0 <= j < len(self.toDest)
+			for x in range(i):
+				assert self.toSend[x] == None
+			for x in range(j):
+				assert self.toDest[x] == -1
+
+
+			if self.toSend[i] != None:
+				print('**Blood has been dispatched**')
+				self._sys.getRoutingSys().sendBlood([self.toSend[i],self.toDest[j]], self.node)
+				self.toSend[i] = None
+				self.toDest[j] = -1
+
+
+			i = i +1
+			j = j + 1
+		self._available = len(self.toSend) -1
+
+		assert self._valid()
+		for i in range(self._size):
+			assert self.toSend[i] == None
+			assert self.toDest[i] == -1
 			
 
 	def setNode(self, node):
