projectVampire/dafny/transportationManager.dfy
@@ -1,23 +1,173 @@
+
+// state:
+// unsafe = -1
+// unverified = 0
+// verified = 1
+// storage = 2
+// dispatched = 3
+// delivered = 4
+
+
+datatype Blood_types = O | A | B | AB
+datatype blood_state = unsafe | unverified | verified | storage | dispatched | delivered
+
+
+// Magic number in expiry time 86400(seconds in day) * 7 =  604800
+class Blood{
+    var state: blood_state;
+    var collection_time: int; //Seconds since Unix Epoch
+    var expiry_time:int
+    var blood_type: Blood_types;
+    var rhesus: bool;
+
+    predicate method Valid()
+    reads this
+    {state== unsafe || state==unverified || state==verified || state==storage || state==dispatched || state==delivered}
+
+    predicate method expired(curr_time:int)
+    reads this
+    {curr_time>expiry_time}
+
+    predicate method safe(curr_time:int)
+    reads this
+    {(state==unverified || state==verified || state==storage || state==dispatched || state==delivered) && !expired(curr_time)}
+
+    method getExpiryTime() returns (expiry : int)
+    // reads this;
+    ensures expiry == expiry_time
+    {
+        expiry := expiry_time;
+        return;
+    }
+
+    method reject_blood()
+    modifies this;
+    ensures state == unsafe
+    ensures Valid()
+    {
+        state := unsafe;
+    }
+
+    method get_blood_type() returns (b_type:Blood_types,rh:bool)
+    ensures b_type==blood_type
+    ensures rh==rhesus
+    {
+        b_type := blood_type;
+        rh := rhesus;
+    }
+
+    method get_state() returns (bl_state:blood_state)
+    ensures bl_state == state
+    {
+        bl_state := state;
+    }
+
+    constructor (secondsin:int)
+    modifies this
+    requires secondsin>=0
+    ensures collection_time>=0 && collection_time==secondsin
+    ensures state == unverified;
+    {
+        collection_time := secondsin;
+        expiry_time:=secondsin + 604800;
+        state := unverified;
+    }
+
+    method verify_blood(curr_time:int,accepted:bool,determined_type:Blood_types,rhesus_in:bool)
+    modifies this;
+    requires state==unverified
+    requires Valid()
+    ensures if (safe(curr_time) && accepted) then state == verified else state==unsafe
+    ensures blood_type==determined_type
+    ensures rhesus == rhesus_in
+    ensures Valid()
+    {
+        if safe(curr_time) && accepted {
+            state:=verified;
+        } else {
+            state:=unsafe;
+        }
+
+        blood_type:=determined_type;
+        rhesus:=rhesus_in;
+    }
+
+    method store_blood(curr_time:int)
+    modifies this
+    requires Valid()
+    requires state==verified;
+    ensures if safe(curr_time) then state == storage else state==unsafe;
+    ensures Valid()
+    {
+        if safe(curr_time) {
+            state:=storage;
+        } else {
+            state:=unsafe;
+        }  
+    }
+
+    method dispatch_blood(curr_time:int)
+    modifies this
+    requires Valid()
+    requires state==storage;
+    ensures if safe(curr_time) then state == dispatched else state==unsafe;
+    ensures Valid()
+    {
+        if safe(curr_time) {
+            state:=dispatched;
+        } else {
+            state:=unsafe;
+        }         
+    }
+
+    method deliver_blood(curr_time:int)
+    modifies this
+    requires Valid()
+    requires state==dispatched;
+    ensures if safe(curr_time) then state ==delivered else state==unsafe;
+    ensures Valid()
+    {
+        if safe(curr_time) {
+            state:=delivered;
+        } else {
+            state:=unsafe;
+        }           
+    }
+
+    method reject()
+    modifies this
+    ensures state ==unsafe;
+    ensures Valid()
+    {state:=unsafe;}
+}
+
+
+
 class transportationManager {
 	
 	var locale: int; // give each location an int value?
+	var available: int;
 	var destinations: array<int>; //:= new int[10]; // routes to destinations
 	var toSend: array<Blood>;// := new Blood[10]; // may need to have another array that matches the blood destinations to each index or create a class that can hold blood and its dest
     	var toDest: array<int>;// := new int[10]; // routes (match with toSend array)
-
+	var size : int;
     	
 
 	// Blood always has a destination, ie every blood in array is matched by a route
 	predicate method Valid()
-	//requires toDest != null;
-	//requires toSend != null
 	reads this;
-	//reads toDest[0],toDest[1], toDest[2],toDest[3],toDest[4],toDest[5],toDest[6],toDest[7],toDest[8],toDest[9];
-	// requires toDest != null;
-	// requires toSend != null;
+	reads this.toDest;
+	reads this.toSend;
+	requires toDest != null;
+	requires toSend != null;
 	{
-        	//forall x,y:: 0 <= x < toDest.Length && 0 <= y < toSend.Length && x == y ==> toDest[x]!=-1 && toSend[y] != null
-    		toDest !=null && toSend != null
+		toDest != null && 
+		toSend != null && 
+		size > 0       && 
+		size == toSend.Length && 
+		size == toDest.Length && 
+		-1 <= available <= size -1 &&
+		forall x :: 0 <= x < size && toSend[x] != null ==> toDest[x] != -1
 	}
 
 
@@ -26,94 +176,60 @@ class transportationManager {
 	modifies toDest;
 	modifies toSend;
 	modifies `locale;
+	modifies `available;
+	modifies `size;
 	requires src >= 0
 	ensures toDest != null;
 	ensures toSend != null;
 	ensures Valid()
 	{
 		locale := src;
-		toDest := new int[10];
-		toSend := new Blood[10];
-		//var i := 0;
-		//assert toSend != null;
-		//while (i < toSend.Length) 
-		//invariant 0 <= i < toSend.Length
-		//{	
-		//	toSend[i] := null;
-		//	i := i + 1;
-		//}
-		//i := 0;
-		//while (i < toDest.Length)
-		//invariant 0 <= i < toDest.Length
-		//{
-		//	toDest[i] := -1;
-		//	i := i + 1;
-		//}
+		size := 10;
+		toDest := new int[size]; // An example amount, could be a different size if required as long as size matches toSend
+		forall x | 0 <= x < toDest.Length {toDest[x] := -1;}
+		toSend := new Blood[size];
+		forall x | 0 <= x < toSend.Length {toSend[x] := null;}
+		available := -1;
+		assert toDest != null;
+		assert toSend != null;
+		var i := 0;
+                var j := 0;
 	}
 
 		
 	method receive(bld:Blood, dst:int)
 	modifies this.toDest
 	modifies this.toSend 
-	requires toSend != null
-	requires toDest != null
+	modifies this`available
+	requires toSend != null;
+	requires toDest != null;
 	requires forall x :: 0 <= x < toSend.Length ==> bld != toSend[x] // blood is not already in toSend
 	requires bld != null;
-	requires toSend.Length == toDest.Length
 	requires dst >= 0;
 	requires Valid(); ensures Valid();
-	//ensures forall x, y:: 0 <= x < toSend.Length && 0 <= y < toDest.Length && x == y ==> toSend[x] == bld && toDest[y] == dst -> need to fix
+	ensures 0 <= available < toSend.Length && 0 <= available < toDest.Length
+	ensures toSend[available] == bld
+	ensures toDest[available] == dst
+	ensures forall x :: 0 <=x < size && x != available ==> toDest[x] == old(toDest)[x]
+	ensures forall x :: 0 <= x < size && x != available ==> toSend[x] == old(toSend)[x]
 	{
-       		var cDest := -1;
-		if (dst == -1) {
-			cDest := 3; // need to grab the dest that system spits out
-		} else {
-			cDest := -1;
-		}
-		//var index := 0;
-		//var i := 0;
-		//while (index < toSend.Length) 
-		//invariant 0 <= i <= toSend.Length
-		//{
-		//	if (toSend[i] == null) {
-		//		index := i;
-		//		i := toSend.Length -1;		
-		//	}
-		//	i :=  i + 1;
-		//}
-		//toSend[i] := bld;
-		//toDest[i] := cDest;
-
-		var i := 0;
-		var j := 0;
-		while (i < toSend.Length && j < toDest.Length)
-		invariant 0 <= i <= toSend.Length
-		invariant 0 <= j <= toDest.Length
-		//invariant forall x,y :: 0 <= x < toSend.Length && 0 <= y < toDest.Length && toDest[y] == cDest && toSend[x] == bld ==> (x==y) -> need to fix
-		//invariant forall x :: 0 <= x < (j-1) ==> toDest[x] != 0
-		//invariant forall x, y :: 0 <= x < i && 0 <= y < j && x == y ==> toSend[x] == bl
-		invariant i == j
-		{
-			if (toSend[i] == null && toDest[j] == 0) {
-				toSend[i] := bld;
-				toDest[j] := cDest;
-				//i := toSend.Length -1;
-				//j := toDest.Length -1;
-			}
-			i := i + 1;
-			j := j + 1;
-		}
-    	}
-
+		
+		available := if available == size -1 then 0 else available + 1;
+		toSend[available] := bld;
+		toDest[available] := dst;
+		
+	}
 
 	method dispatchBlood()
-	modifies toSend;
-	modifies toDest;
+	modifies this.toSend;
+	modifies this.toDest;
+	modifies this`available;
 	requires toSend != null;
 	requires toDest != null;
 	requires exists x :: 0 <= x < toSend.Length && toSend[x] != null // blood is to be sent
-	requires Valid();ensures Valid();
-    	ensures forall x, y:: 0 <= x < toSend.Length && 0 <= y < toDest.Length  && x == y ==> (toSend[x] == null && toDest[y] == 0) // toSend and toRoute are empty
+	requires Valid();
+	ensures Valid();
+    	ensures forall x, y:: 0 <= x < toSend.Length && 0 <= y < toDest.Length  && x == y ==> (toSend[x] == null && toDest[y] == -1) // toSend and toRoute are empty
 	{
 		var i := 0;
 		var j := 0;
@@ -121,15 +237,16 @@ class transportationManager {
 		invariant 0 <= i <= toSend.Length
 		invariant 0 <= j <= toDest.Length
 		invariant forall x :: 0 <= x < i ==> toSend[x] == null
-		invariant forall x :: 0 <= x < j ==> toDest[x] == 0
+		invariant forall x :: 0 <= x < j ==> toDest[x] == -1
 		invariant i == j
 		{
-			toDest[j] := 0;
+			// dispatch
+			toDest[j] := -1;
 			toSend[i] := null;
 			i := i + 1;
 			j := j + 1;
 		}
-		
+		available := toSend.Length -1;	
     	}
     
 }
